Primops module

src/zksync_verifier.ec
@@ -1,125 +1,33 @@
 pragma Goals:printall.
-require import Int Logic IntDiv CoreMap SmtMap Array.
 
-type uint256 = int.
-type mem = (uint256, uint256) map.
+require import Logic UInt256 Memory YulPrimops Array.
 
 op p = 21888242871839275222246405745257275088696311157297823662689037894645226208583.
-op calldata : uint256 array.
 
 module Test = {
-
-  proc mload(a : uint256, m : mem) : uint256 = {
-    return m.[a];
-  }
-
-  proc mstore(a : uint256, v : uint256, m : mem) : mem = {
-    return m.[a<-v];
-  }
-
-  proc mstore8(a : uint256, v : uint256, m : mem) : mem = {
-    (* TODO: memory model? *)
-    return m;
-  }
-
-  proc staticcall(gas : uint256, addr : uint256, argOff : uint256, argSize : uint256, retOff : uint256, retSize : uint256, m : mem) : uint256 * mem = {
-    var succ, m';
-    if (addr = 5) {
-      (* TODO: modexp *)
-      succ <- 0;
-      m' <- m;
-    } else {
-      if (addr = 6) {
-        (* TODO: ecAdd *)
-        succ <- 0;
-        m' <- m;
-      } else {
-        if (addr = 7) {
-          (* TODO: ecMul *)
-          succ <- 0;
-          m' <- m;
-        } else {
-          if (addr = 8) {
-            (* TODO: ecPairing *)
-            succ <- 0;
-            m' <- m;
-          } else {
-              succ <- 0;
-              m' <- m;
-          }
-        }
-      }
-    }
-    return (succ, m');
-  }  
-
-  proc revert() : unit = {
-    (* TODO: Implement revert, needs to be differentiable from return *)
-    return ();
-  }
-
-  proc calldataload(i : uint256) : uint256 = {
-    return calldata.[i];
-  }
-  
-  proc calldatasize(i : uint256) : uint256 = {
-    return size(calldata);
-  }
-
-  proc ret(retOff : uint256, retSize : uint256) : unit = {
-    (* TODO: Implement return, needs to be differentiable from revert *)
-    return ();
-  }
-  
-  proc gas() : uint256 = {
-    (* Confirm ok *)
-    return 42;
-  }
-  
-  proc iszero(v : uint256) : uint256 = {
-    var ref;
-    if (v = 0) {
-      ref <- 1;
-    } else {
-      ref <- 0;
-    }
-    return ref;
-  }
-
-  proc mulmod(a : uint256, b : uint256, n : uint256) : uint256 = {
-    return (a * b) %% n;
-  }
-
-  proc addmod(a : uint256, b : uint256, n : uint256) : uint256 = {
-    return (a + b) %% n;
-  }
-
-  proc keccak256(v : uint256) : uint256 = {
-    (* TODO: return sample from uniform distribution over uint256 *)
-    return 0;
-  }
-  
+    
   proc pointNegate(m : mem, point : uint256) : mem = {
       var _1, _2, _3, pY, tmp166, tmp167, tmp168, _6, _7, tmp170;
+      Primops.m <- m;
       _1 <- 32;
       _2 <- point + _1;
-      tmp166 <@ mload(_2, m);
+      tmp166 <@ Primops.mload(_2);
       pY <- tmp166;
       tmp167 <- pY;
       if (tmp167 = 0)
       {
-        tmp168 <@ mload(point, m);
+        tmp168 <@ Primops.mload(point);
         _3 <- tmp168;
         if (_3 = 0)
         {
         }
-        tmp170 <- m;
+        (* tmp170 <- Primops.m; *)
       } else {
           _6 <- 21888242871839275222246405745257275088696311157297823662689037894645226208583;
           _7 <- _6 - pY;
-          tmp170 <@ mstore(_2, _7, m);
+          tmp170 <@ Primops.mstore(_2, _7);
       } 
-      return tmp170;
+      return Primops.m;
     }
   
 }.
@@ -151,8 +59,8 @@ lemma pointNegate_correctness :
             progress.
             proc.
             simplify.
-            inline Test.mload.
-            inline Test.mstore.
+            inline Primops.mload.
+            inline Primops.mstore.
             wp.
             skip.
             progress.
