src/Memory.ec
@@ -1,0 +1,4 @@
+require import UInt256.
+require export CoreMap SmtMap.
+
+type mem = (uint256, uint256) map.
