src/UInt256.ec
@@ -1,0 +1,5 @@
+pragma Goals:printall.
+
+require export Int IntDiv.
+
+type uint256 = int.
