src/YulPrimops.ec
@@ -1,0 +1,96 @@
+pragma Goals:printall.
+
+require import Logic Array.
+require export UInt256 Memory.
+
+op calldata : uint256 array.
+
+module Primops = {
+  var m : mem
+
+  proc mload(a : uint256) : uint256 = { 
+    return m.[a];
+  }
+
+  proc mstore(a : uint256, v : uint256): unit = {
+    m <- m.[a<-v];
+  }
+
+  proc mstore8(a : uint256, v : uint256) : uint256 = {
+    (* TODO: memory model? *)
+    return m.[a];
+  }
+
+  proc ret(retOff : uint256, retSize : uint256) : unit = {
+    (* TODO: Implement return, needs to be differentiable from revert *)
+    return ();
+  }
+  
+  proc gas() : uint256 = {
+    (* Confirm ok *)
+    return 42;
+  }
+  
+  proc iszero(v : uint256) : uint256 = {
+    var ref;
+    if (v = 0) {
+      ref <- 1;
+    } else {
+      ref <- 0;
+    }
+    return ref;
+  }
+
+  proc mulmod(a : uint256, b : uint256, n : uint256) : uint256 = {
+    return (a * b) %% n;
+  }
+
+  proc addmod(a : uint256, b : uint256, n : uint256) : uint256 = {
+    return (a + b) %% n;
+  }
+
+  proc keccak256(v : uint256) : uint256 = {
+    (* TODO: return sample from uniform distribution over uint256 *)
+    return 0;
+  }
+
+  proc staticcall(gas : uint256, addr : uint256, argOff : uint256, argSize : uint256, retOff : uint256, retSize : uint256, m : mem) : uint256 * mem = {
+    var succ, m';
+    if (addr = 5) {
+      (* TODO: modexp *)
+      succ <- 0;
+      m' <- m;
+    } else {
+      if (addr = 6) {
+        (* TODO: ecAdd *)
+        succ <- 0;
+        m' <- m;
+      } else {
+        if (addr = 7) {
+          (* TODO: ecMul *)
+          succ <- 0;
+          m' <- m;
+        } else {
+          if (addr = 8) {
+            (* TODO: ecPairing *)
+            succ <- 0;
+            m' <- m;
+          } else {
+              succ <- 0;
+              m' <- m;
+          }
+        }
+      }
+    }
+    return (succ, m');
+  }  
+
+  proc revert() : unit = {
+    (* TODO: Implement revert, needs to be differentiable from return *)
+    return ();
+  }
+
+  proc calldataload(i : uint256) : uint256 = {
+    return calldata.[i];
+  }
+}.
